Split the MEM type class into MemOps and MemSpec
This makes it easier to define new instances: define the operations
first, then prove things about them. More generally, it makes sense to
separate the code, which should be transparent and will be extracted,
from the associated proofs, which can be opaque and will be erased.

Nevertheless, for now MemSpec is still in Type rather than Prop because
some fields are informative (ie. use [sig] rather that [exists]).

common/Memtype.v
@@ -85,7 +85,7 @@ Inductive perm_kind: Type :=
 
 Module Mem.
 
-Class MEM (mem: Type) := {
+Class MemOps (mem: Type) := {
 
 nullptr: block := 0;
 
@@ -93,6 +93,10 @@ nullptr: block := 0;
 
 (** [empty] is the initial memory state. *)
 empty: mem;
+
+(** The next block of a memory state is the block identifier for the
+  next allocation.  It increases by one at each allocation. *)
+nextblock: mem -> block;
 
 (** [alloc m lo hi] allocates a fresh block of size [hi - lo] bytes.
   Valid offsets in this block are between [lo] included and [hi] excluded.
@@ -157,38 +161,97 @@ free_list := fix free_list (m: mem) (l: list (block * Z * Z)) {struct l}: option
       end
   end;
 
-(** [drop_perm m b lo hi p] sets the permissions of the byte range
-    [(b, lo) ... (b, hi - 1)] to [p].  These bytes must have [Freeable] permissions
-    in the initial memory state [m].
-    Returns updated memory state, or [None] if insufficient permissions. *)
-
-drop_perm: forall (m: mem) (b: block) (lo hi: Z) (p: permission), option mem;
-
-(** * Permissions, block validity, access validity, and bounds *)
-
-(** The next block of a memory state is the block identifier for the
-  next allocation.  It increases by one at each allocation.
-  Block identifiers below [nextblock] are said to be valid, meaning
-  that they have been allocated previously.  Block identifiers above
-  [nextblock] are fresh or invalid, i.e. not yet allocated.  Note that
-  a block identifier remains valid after a [free] operation over this
-  block. *)
-
-nextblock: mem -> block;
-nextblock_pos m:
-  nextblock m > 0;
-
-valid_block (m: mem) (b: block) :=
-  b < nextblock m;
-valid_not_valid_diff m b b':
-  valid_block m b -> ~(valid_block m b') -> b <> b';
-
 (** [perm m b ofs k p] holds if the address [b, ofs] in memory state [m]
   has permission [p]: one of freeable, writable, readable, and nonempty.
   If the address is empty, [perm m b ofs p] is false for all values of [p].
   [k] is the kind of permission we are interested in: either the current
   permissions or the maximal permissions. *)
 perm: forall (m: mem) (b: block) (ofs: Z) (k: perm_kind) (p: permission), Prop;
+
+(** [valid_pointer m b ofs] returns [true] if the address [b, ofs]
+  is nonempty in [m] and [false] if it is empty. *)
+valid_pointer: forall (m: mem) (b: block) (ofs: Z), bool;
+
+(** [drop_perm m b lo hi p] sets the permissions of the byte range
+    [(b, lo) ... (b, hi - 1)] to [p].  These bytes must have [Freeable] permissions
+    in the initial memory state [m].
+    Returns updated memory state, or [None] if insufficient permissions. *)
+drop_perm: forall (m: mem) (b: block) (lo hi: Z) (p: permission), option mem;
+
+(**  A store [m2] extends a store [m1] if [m2] can be obtained from [m1]
+  by relaxing the permissions of [m1] (for instance, allocating larger
+  blocks) and replacing some of the [Vundef] values stored in [m1] by
+  more defined values stored in [m2] at the same addresses. *)
+extends: mem -> mem -> Prop;
+
+(** A memory injection [f] is a function from addresses to either [None]
+  or [Some] of an address and an offset.  It defines a correspondence
+  between the blocks of two memory states [m1] and [m2]:
+  - if [f b = None], the block [b] of [m1] has no equivalent in [m2];
+  - if [f b = Some(b', ofs)], the block [b] of [m2] corresponds to
+    a sub-block at offset [ofs] of the block [b'] in [m2].
+
+  A memory injection [f] defines a relation [val_inject] between values
+  that is the identity for integer and float values, and relocates pointer 
+  values as prescribed by [f].  (See module [Values].)
+
+  Likewise, a memory injection [f] defines a relation between memory states 
+  that we axiomatize below. *)
+inject: meminj -> mem -> mem -> Prop;
+
+(** Memory states that inject into themselves. *)
+inject_neutral: forall (thr: block) (m: mem), Prop
+
+}.
+
+Section MEMOPS_DEFS.
+
+Context `{mem_ops: MemOps}.
+
+(** Block identifiers below [nextblock] are said to be valid, meaning
+  that they have been allocated previously.  Block identifiers above
+  [nextblock] are fresh or invalid, i.e. not yet allocated.  Note that
+  a block identifier remains valid after a [free] operation over this
+  block. *)
+Definition valid_block (m: mem) (b: block) :=
+  b < nextblock m.
+
+(** [range_perm m b lo hi p] holds iff the addresses [b, lo] to [b, hi-1]
+  all have permission [p] of kind [k]. *)
+Definition range_perm (m: mem) (b: block) (lo hi: Z) (k: perm_kind) (p: permission) : Prop :=
+  forall ofs, lo <= ofs < hi -> perm m b ofs k p.
+
+(** An access to a memory quantity [chunk] at address [b, ofs] with
+  permission [p] is valid in [m] if the accessed addresses all have
+  current permission [p] and moreover the offset is properly aligned. *)
+Definition valid_access (m: mem) (chunk: memory_chunk) (b: block) (ofs: Z) (p: permission): Prop :=
+  range_perm m b ofs (ofs + size_chunk chunk) Cur p
+  /\ (align_chunk chunk | ofs).
+
+(** C allows pointers one past the last element of an array.  These are not
+  valid according to the previously defined [valid_pointer]. The property
+  [weak_valid_pointer m b ofs] holds if address [b, ofs] is a valid pointer
+  in [m], or a pointer one past a valid block in [m].  *)
+Definition weak_valid_pointer (m: mem) (b: block) (ofs: Z) :=
+  valid_pointer m b ofs || valid_pointer m b (ofs - 1).
+
+End MEMOPS_DEFS.
+
+Definition inj_offset_aligned (delta: Z) (size: Z) : Prop :=
+  forall chunk, size_chunk chunk <= size -> (align_chunk chunk | delta).
+
+Definition flat_inj (thr: block) : meminj :=
+  fun (b: block) => if zlt b thr then Some(b, 0) else None.
+
+Class MemSpec (mem: Type) `{mem_ops: MemOps mem} := {
+
+(** * Permissions, block validity, access validity, and bounds *)
+
+nextblock_pos m:
+  nextblock m > 0;
+
+valid_not_valid_diff m b b':
+  valid_block m b -> ~(valid_block m b') -> b <> b';
 
 (** Logical implications between permissions *)
 
@@ -213,11 +276,6 @@ perm_valid_block m b ofs k p:
 perm_dec m b ofs k p:
   {perm m b ofs k p} + {~ perm m b ofs k p};
 
-(** [range_perm m b lo hi p] holds iff the addresses [b, lo] to [b, hi-1]
-  all have permission [p] of kind [k]. *)
-range_perm (m: mem) (b: block) (lo hi: Z) (k: perm_kind) (p: permission) : Prop :=
-  forall ofs, lo <= ofs < hi -> perm m b ofs k p;
-
 range_perm_implies m b lo hi k p1 p2:
   range_perm m b lo hi k p1 -> perm_order p1 p2 -> range_perm m b lo hi k p2;
 range_perm_cur:
@@ -226,13 +284,6 @@ range_perm_cur:
 range_perm_max:
   forall m b lo hi k p,
   range_perm m b lo hi k p -> range_perm m b lo hi Max p;
-
-(** An access to a memory quantity [chunk] at address [b, ofs] with
-  permission [p] is valid in [m] if the accessed addresses all have
-  current permission [p] and moreover the offset is properly aligned. *)
-valid_access (m: mem) (chunk: memory_chunk) (b: block) (ofs: Z) (p: permission): Prop :=
-  range_perm m b ofs (ofs + size_chunk chunk) Cur p
-  /\ (align_chunk chunk | ofs);
 
 valid_access_implies m chunk b ofs p1 p2:
   valid_access m chunk b ofs p1 -> perm_order p1 p2 ->
@@ -249,20 +300,10 @@ valid_access_perm m chunk b ofs k p:
 (** [valid_pointer m b ofs] returns [true] if the address [b, ofs]
   is nonempty in [m] and [false] if it is empty. *)
 
-valid_pointer: forall (m: mem) (b: block) (ofs: Z), bool;
-
 valid_pointer_nonempty_perm m b ofs:
   valid_pointer m b ofs = true <-> perm m b ofs Cur Nonempty;
 valid_pointer_valid_access m b ofs:
   valid_pointer m b ofs = true <-> valid_access m Mint8unsigned b ofs Nonempty;
-
-(** C allows pointers one past the last element of an array.  These are not
-  valid according to the previously defined [valid_pointer]. The property
-  [weak_valid_pointer m b ofs] holds if address [b, ofs] is a valid pointer
-  in [m], or a pointer one past a valid block in [m].  *)
-
-weak_valid_pointer (m: mem) (b: block) (ofs: Z) :=
-  valid_pointer m b ofs || valid_pointer m b (ofs - 1);
 
 weak_valid_pointer_spec m b ofs:
   weak_valid_pointer m b ofs = true <->
@@ -780,13 +821,6 @@ load_drop m b lo hi p m':
 
 (** ** Memory extensions *)
 
-(**  A store [m2] extends a store [m1] if [m2] can be obtained from [m1]
-  by relaxing the permissions of [m1] (for instance, allocating larger
-  blocks) and replacing some of the [Vundef] values stored in [m1] by
-  more defined values stored in [m2] at the same addresses. *)
-
-extends: mem -> mem -> Prop;
-
 extends_refl m:
   extends m m;
 
@@ -884,22 +918,6 @@ weak_valid_pointer_extends m1 m2 b ofs:
   weak_valid_pointer m1 b ofs = true -> weak_valid_pointer m2 b ofs = true;
 
 (** * Memory injections *)
-
-(** A memory injection [f] is a function from addresses to either [None]
-  or [Some] of an address and an offset.  It defines a correspondence
-  between the blocks of two memory states [m1] and [m2]:
-- if [f b = None], the block [b] of [m1] has no equivalent in [m2];
-- if [f b = Some(b', ofs)], the block [b] of [m2] corresponds to
-  a sub-block at offset [ofs] of the block [b'] in [m2].
-
-A memory injection [f] defines a relation [val_inject] between values
-that is the identity for integer and float values, and relocates pointer 
-values as prescribed by [f].  (See module [Values].)
-
-Likewise, a memory injection [f] defines a relation between memory states 
-that we now axiomatize. *)
-
-inject: meminj -> mem -> mem -> Prop;
 
 mi_freeblocks f m1 m2:
   inject f m1 m2 ->
@@ -1106,9 +1124,6 @@ alloc_left_unmapped_inject f m1 m2 lo hi m1' b1:
   /\ f' b1 = None
   /\ (forall b, b <> b1 -> f' b = f b);
 
-inj_offset_aligned (delta: Z) (size: Z) : Prop :=
-  forall chunk, size_chunk chunk <= size -> (align_chunk chunk | delta);
-
 alloc_left_mapped_inject f m1 m2 lo hi m1' b1 b2 delta:
   inject f m1 m2 ->
   alloc m1 lo hi = (m1', b1) ->
@@ -1184,11 +1199,6 @@ drop_outside_inject f m1 m2 b lo hi p m2':
   inject f m1 m2';
 
 (** Memory states that inject into themselves. *)
-
-flat_inj (thr: block) : meminj :=
-  fun (b: block) => if zlt b thr then Some(b, 0) else None;
-
-inject_neutral: forall (thr: block) (m: mem), Prop;
 
 neutral_inject m:
   inject_neutral (nextblock m) m ->
